theories/transaction.v
@@ -1,0 +1,164 @@
+From iris.algebra Require Import auth gmap gset.
+From iris.proofmode Require Import tactics.
+From HypVeri Require Import monad.
+From HypVeri Require Export lang machine RAs.
+
+
+  Definition serialized_memory_descirptor l (r:VMID) ps := [l; (of_imm (encode_vmid r))]++ (map (λ pid, (of_pid pid)) ps).
+
+  Definition serialized_transaction_descriptor (v r:VMID) (wf  l : Word) (ps: list PID) (h : handle ): list Word :=
+    [(of_imm (encode_vmid v)); wf; h] ++ (serialized_memory_descirptor l r ps).
+
+  Lemma trans_desc_length{i j wf l ps} des :
+    des = serialized_transaction_descriptor i j wf  l ps W0 ->
+    (finz.to_z l) = (Z.of_nat (length ps)) ->
+    ((Z.of_nat (length des)) = 5 + (finz.to_z l))%Z.
+  Proof.
+    intros.
+    rewrite H /serialized_transaction_descriptor /serialized_memory_descirptor H0.
+    simpl.
+    rewrite fmap_length.
+    lia.
+  Qed.
+
+
+  Lemma mem_desc_valid{ b psd σ}l ps:
+    l =  (length ps) ->
+   psd =  (map (λ pid, (of_pid pid)) ps) ->
+   (∀ (k : nat) (y1 y2 : Addr),
+   finz.seq b (length psd) !! k = Some y1 → psd !! k = Some y2 → get_mem σ !! y1 = Some y2) ->
+   map (λ v : Addr,(bind ((get_mem σ) !! v) to_pid )) (finz.seq b l)
+   = map (λ pid, Some pid) ps.
+  Proof.
+    intros.
+    generalize dependent b.
+    generalize dependent ps.
+    generalize dependent psd.
+    induction l.
+    intros.
+    destruct ps .
+    rewrite H //=.
+    simplify_eq.
+    intros.
+    destruct ps .
+    done.
+    simpl in H.
+    inversion H.
+    simpl.
+    destruct psd.
+    done.
+    rewrite -(IHl psd _ _ _ (b^+1)%f).
+    pose proof (H1 0 b (of_pid p)).
+    rewrite H2.
+    rewrite H3 to_of_pid //.
+    done.
+    rewrite H0.
+    rewrite -> list_lookup_fmap.
+    done.
+    done.
+    rewrite -> fmap_cons in H0.
+    inversion H0.
+    done.
+    intros.
+    apply (H1 (k+1)).
+    simpl.
+    rewrite lookup_cons_ne_0.
+    rewrite -H2 //=.
+    f_equal.
+    lia.
+    lia.
+    rewrite -H4.
+    rewrite lookup_cons_ne_0.
+    f_equal.
+    lia.
+    lia.
+  Qed.
+
+  Definition transaction_l (v r:VMID) (wf: Word) (b:bool) (r:  VMID) (ps: list PID)  (ty: transaction_type): transaction :=
+    (v,wf,b,r ,(list_to_set ps),ty).
+
+  Lemma sequence_a_map_unit{A} (l:list A) :
+  @sequence_a list _ _ _ A option _ _ (map (λ e , Some e ) l) = Some l.
+    Proof.
+      unfold sequence_a.
+      simpl.
+      unfold monad.List.sequence_a_list.
+      induction l.
+      done.
+      simpl.
+      simpl in IHl.
+      rewrite IHl //.
+Qed.
+
+  Lemma transaction_descriptor_valid{i j wf l psd σ} des p :
+    (finz.to_z l) = (Z.of_nat (length psd)) ->
+    des = serialized_transaction_descriptor i j wf l psd W0 ->
+    seq_in_page (of_pid p) (length des) p ->
+   (∀ (k : nat) (y1 y2 : Addr),
+             finz.seq (of_pid p) (length des) !! k = Some y1 → des !! k = Some y2 → get_mem σ !! y1 = Some y2) ->
+   parse_transaction_descriptor σ p = Some (i , None, wf,  j , (list_to_set  psd)).
+  Proof.
+    intros.
+    rewrite /parse_transaction_descriptor /get_memory_with_offset.
+    destruct H1 as [_ [? _]].
+    pose proof (trans_desc_length des H0 H) as Hlen.
+    assert (HpSome: ((of_pid p) + 0)%f = Some ((of_pid p) ^+ 0)%f).
+    solve_finz.
+    rewrite HpSome //=;clear HpSome.
+    rewrite (H2 0 ((of_pid p) ^+ 0)%f (encode_vmid i)).
+    2: { apply finz_seq_lookup. lia. solve_finz. }
+    2: { rewrite H0 /serialized_transaction_descriptor. by list_simplifier. }
+    assert (HpSome: ((of_pid p) + 1)%f = Some ((of_pid p) ^+ 1)%f).
+    solve_finz.
+    rewrite HpSome //=;clear HpSome.
+    rewrite (H2 1 ((of_pid p) ^+ 1)%f wf).
+    2: { apply finz_seq_lookup. lia. solve_finz. }
+    2: { rewrite H0 /serialized_transaction_descriptor. by list_simplifier. }
+    assert (HpSome: ((of_pid p) + 2)%f = Some ((of_pid p) ^+ 2)%f).
+    solve_finz.
+    rewrite HpSome //=;clear HpSome.
+    rewrite (H2 2 ((of_pid p) ^+ 2)%f W0).
+    2: { apply finz_seq_lookup. lia. solve_finz. }
+    2: { rewrite H0 /serialized_transaction_descriptor. by list_simplifier. }
+    rewrite  /parse_memory_region_descriptor /get_memory_with_offset.
+    assert (HpSome: ((of_pid p) ^+ 3 + 0)%f = Some ((of_pid p) ^+ 3)%f).
+    solve_finz.
+    rewrite HpSome //=;clear HpSome.
+    rewrite (H2 3 ((of_pid p) ^+ 3)%f l).
+    2: { apply finz_seq_lookup. lia. solve_finz. }
+    2: { rewrite H0 /serialized_transaction_descriptor. by list_simplifier. }
+    assert (HpSome: ((of_pid p) ^+ 3 + 1)%f = Some ((of_pid p) ^+ 4)%f).
+    solve_finz.
+    rewrite HpSome //=;clear HpSome.
+    rewrite (H2 4 ((of_pid p) ^+ 4)%f (encode_vmid j)).
+    2: { apply finz_seq_lookup. lia. solve_finz. }
+    2: { rewrite H0 /serialized_transaction_descriptor. by list_simplifier. }
+    rewrite !decode_encode_vmid /parse_list_of_pids /= .
+    rewrite (@mem_desc_valid _ (map (λ pid, (of_pid pid)) psd) _ _ psd );eauto.
+    2: { lia. }
+    2: { intros.
+         apply (H2 (k+5) _).
+         assert (Hlenmapeq: length ( map (λ pid : PID, (of_pid pid)) psd) = length psd).
+        apply fmap_length.
+         apply (finz_seq_lookup _ _ y1).
+         assert (Hklt: k < length ( map (λ pid : PID, (of_pid pid)) psd)).
+         rewrite <-(finz_seq_length _ ((p ^+ 3) ^+ 2)%f).
+         apply lookup_lt_is_Some.
+         by exists y1.
+        rewrite Hlenmapeq in Hklt.
+        lia.
+        apply (finz_seq_lookup'  _ y1 k _ ) in H3.
+        2: { rewrite Hlenmapeq. solve_finz. }
+        destruct H3.
+        rewrite Hlenmapeq in H3.
+        solve_finz.
+        rewrite H0 /serialized_transaction_descriptor.
+        simpl.
+        rewrite !lookup_cons_ne_0; try lia.
+        rewrite -H4.
+        f_equal.
+        lia.
+       }
+    rewrite -> sequence_a_map_unit.
+    done.
+ Qed.
